Move finite set and cardinality results from Exponential_Objects to Nats

Nats.thy
@@ -159,6 +159,490 @@ proof -
     by auto
 qed
 
+section \<open>Cardinality and Finiteness\<close>
+
+text \<open>The definitions below correspond to Definition 2.6.1 in Halvorson\<close>
+definition is_finite :: "cset \<Rightarrow> bool"  where
+   "is_finite(X) \<longleftrightarrow> (\<forall>m. (m : X \<rightarrow> X \<and> monomorphism(m)) \<longrightarrow>  isomorphism(m))"
+
+definition is_infinite :: "cset \<Rightarrow> bool"  where
+   "is_infinite(X) \<longleftrightarrow> (\<exists> m. (m : X \<rightarrow> X \<and> monomorphism(m) \<and> \<not>surjective(m)))"
+
+lemma either_finite_or_infinite:
+  "is_finite(X) \<or> is_infinite(X)"
+  using epi_mon_is_iso is_finite_def is_infinite_def surjective_is_epimorphism by blast
+
+text \<open>The definition below corresponds to Definition 2.6.2 in Halvorson\<close>
+definition is_smaller_than :: "cset \<Rightarrow> cset \<Rightarrow> bool" (infix "\<le>\<^sub>c" 50) where
+   "X \<le>\<^sub>c Y \<longleftrightarrow> (\<exists> m. m : X \<rightarrow> Y \<and> monomorphism(m))"
+
+text \<open>The purpose of the following lemma is simply to unify the two notations used in the book.\<close>
+lemma subobject_iff_smaller_than:
+  "(X \<le>\<^sub>c Y) = (\<exists>m. (X,m) \<subseteq>\<^sub>c Y)"
+  using is_smaller_than_def subobject_of_def2 by auto
+
+lemma set_card_transitive:
+  assumes "A \<le>\<^sub>c B"
+  assumes "B \<le>\<^sub>c C"
+  shows   "A \<le>\<^sub>c C"
+  by (typecheck_cfuncs, metis (full_types) assms cfunc_type_def comp_type composition_of_monic_pair_is_monic is_smaller_than_def)
+
+lemma all_emptysets_are_finite:
+  assumes "is_empty X"
+  shows "is_finite(X)"
+  by (metis assms epi_mon_is_iso epimorphism_def3 is_finite_def is_empty_def one_separator)
+
+lemma emptyset_is_smallest_set:
+  "\<emptyset> \<le>\<^sub>c X"
+  using empty_subset is_smaller_than_def subobject_of_def2 by auto
+
+lemma truth_set_is_finite:
+  "is_finite \<Omega>"
+  unfolding is_finite_def
+proof(auto)
+  fix m 
+  assume m_type[type_rule]: "m : \<Omega> \<rightarrow> \<Omega>"
+  assume m_mono: "monomorphism(m)"
+  have "surjective(m)"
+    unfolding surjective_def
+  proof(auto)
+    fix y
+    assume "y \<in>\<^sub>c codomain m" 
+    then have "y \<in>\<^sub>c \<Omega>"
+      using cfunc_type_def m_type by force
+    show "\<exists>x. x \<in>\<^sub>c domain m \<and> m \<circ>\<^sub>c x = y"
+      by (smt (verit, del_insts) \<open>y \<in>\<^sub>c \<Omega>\<close> cfunc_type_def codomain_comp domain_comp injective_def m_mono m_type monomorphism_imp_injective true_false_only_truth_values)
+  qed
+  then show "isomorphism m"
+    by (simp add: epi_mon_is_iso m_mono surjective_is_epimorphism)
+qed
+
+lemma smaller_than_finite_is_finite:
+  assumes "X \<le>\<^sub>c Y" "is_finite Y" 
+  shows "is_finite X"
+  unfolding is_finite_def
+proof(auto)
+  fix x
+  assume x_type: "x : X \<rightarrow> X"
+  assume x_mono: "monomorphism x"
+
+  obtain m where m_def: "m: X \<rightarrow> Y \<and> monomorphism m"
+    using assms(1) is_smaller_than_def by blast
+  obtain \<phi> where \<phi>_def: "\<phi> = into_super m \<circ>\<^sub>c (x \<bowtie>\<^sub>f id(Y \<setminus> (X,m))) \<circ>\<^sub>c try_cast m" 
+    by auto
+
+  have \<phi>_type: "\<phi> : Y \<rightarrow> Y"
+    unfolding \<phi>_def
+    using x_type m_def by (typecheck_cfuncs, blast)
+
+  have "injective(x \<bowtie>\<^sub>f id(Y \<setminus> (X,m)))"
+    using cfunc_bowtieprod_inj id_isomorphism id_type iso_imp_epi_and_monic monomorphism_imp_injective x_mono x_type by blast
+  then have mono1: "monomorphism(x \<bowtie>\<^sub>f id(Y \<setminus> (X,m)))"
+    using injective_imp_monomorphism by auto
+  have mono2: "monomorphism(try_cast m)"
+    using m_def try_cast_mono by blast
+  have mono3: "monomorphism((x \<bowtie>\<^sub>f id(Y \<setminus> (X,m))) \<circ>\<^sub>c try_cast m)"
+    using cfunc_type_def composition_of_monic_pair_is_monic m_def mono1 mono2 x_type by (typecheck_cfuncs, auto)
+  then have \<phi>_mono: "monomorphism(\<phi>)" 
+    unfolding \<phi>_def
+    using cfunc_type_def composition_of_monic_pair_is_monic 
+          into_super_mono m_def mono3 x_type by (typecheck_cfuncs,auto)
+  then have "isomorphism(\<phi>)" 
+    using \<phi>_def \<phi>_type assms(2) is_finite_def by blast
+  have iso_x_bowtie_id: "isomorphism(x \<bowtie>\<^sub>f id(Y \<setminus> (X,m)))"
+    by (typecheck_cfuncs, smt \<open>isomorphism \<phi>\<close> \<phi>_def comp_associative2 id_left_unit2 into_super_iso into_super_try_cast into_super_type isomorphism_sandwich m_def try_cast_type x_type)
+  have "left_coproj X (Y \<setminus> (X,m)) \<circ>\<^sub>c x = (x \<bowtie>\<^sub>f id(Y \<setminus> (X,m))) \<circ>\<^sub>c left_coproj X (Y \<setminus> (X,m))"
+    using x_type  
+    by (typecheck_cfuncs, simp add: left_coproj_cfunc_bowtie_prod)
+  have "epimorphism(x \<bowtie>\<^sub>f id(Y \<setminus> (X,m)))"
+    using iso_imp_epi_and_monic iso_x_bowtie_id by blast
+  then have "surjective(x \<bowtie>\<^sub>f id(Y \<setminus> (X,m)))"
+    using  epi_is_surj x_type by (typecheck_cfuncs, blast)
+  then have "epimorphism(x)"
+    using x_type cfunc_bowtieprod_surj_converse id_type surjective_is_epimorphism by blast
+  then show "isomorphism(x)"
+    by (simp add: epi_mon_is_iso x_mono)
+qed
+
+lemma larger_than_infinite_is_infinite:
+  assumes "X \<le>\<^sub>c Y" "is_infinite(X)" 
+  shows "is_infinite(Y)"
+  using assms either_finite_or_infinite epi_is_surj is_finite_def is_infinite_def
+    iso_imp_epi_and_monic smaller_than_finite_is_finite by blast
+
+text \<open>The next two lemmas below correspond to Proposition 2.6.3 in Halvorson\<close>
+lemma smaller_than_coproduct1:
+  "X \<le>\<^sub>c X \<Coprod> Y"
+  using is_smaller_than_def left_coproj_are_monomorphisms left_proj_type by blast
+
+lemma  smaller_than_coproduct2:
+  "X \<le>\<^sub>c Y \<Coprod> X"
+  using is_smaller_than_def right_coproj_are_monomorphisms right_proj_type by blast
+
+text \<open>The next two lemmas below correspond to Proposition 2.6.4 in Halvorson\<close>
+lemma smaller_than_product1:
+  assumes "nonempty Y"
+  shows "X \<le>\<^sub>c X \<times>\<^sub>c Y"
+  unfolding is_smaller_than_def  
+proof-
+  obtain y where y_type: "y \<in>\<^sub>c Y"
+  using assms nonempty_def by blast
+  have map_type: "\<langle>id(X),y \<circ>\<^sub>c \<beta>\<^bsub>X\<^esub>\<rangle> : X \<rightarrow> X \<times>\<^sub>c Y"
+   using y_type cfunc_prod_type cfunc_type_def codomain_comp domain_comp id_type terminal_func_type by auto
+  have mono: "monomorphism(\<langle>id X, y \<circ>\<^sub>c \<beta>\<^bsub>X\<^esub>\<rangle>)"
+    using map_type
+  proof (unfold monomorphism_def3, auto)
+    fix g h A
+    assume g_h_types: "g : A \<rightarrow> X" "h : A \<rightarrow> X"
+    
+    assume "\<langle>id\<^sub>c X,y \<circ>\<^sub>c \<beta>\<^bsub>X\<^esub>\<rangle> \<circ>\<^sub>c g = \<langle>id\<^sub>c X,y \<circ>\<^sub>c \<beta>\<^bsub>X\<^esub>\<rangle> \<circ>\<^sub>c h"
+    then have "\<langle>id\<^sub>c X \<circ>\<^sub>c g, y \<circ>\<^sub>c \<beta>\<^bsub>X\<^esub> \<circ>\<^sub>c g\<rangle>  = \<langle>id\<^sub>c X \<circ>\<^sub>c h, y \<circ>\<^sub>c \<beta>\<^bsub>X\<^esub> \<circ>\<^sub>c h\<rangle>"
+      using y_type g_h_types by (typecheck_cfuncs, smt cfunc_prod_comp comp_associative2 comp_type)
+    then have "\<langle>g, y \<circ>\<^sub>c \<beta>\<^bsub>A\<^esub>\<rangle>  = \<langle>h, y \<circ>\<^sub>c \<beta>\<^bsub>A\<^esub>\<rangle>"
+      using y_type g_h_types id_left_unit2 terminal_func_comp by (typecheck_cfuncs, auto)
+    then show "g = h"
+      using g_h_types y_type
+      by (metis (full_types) comp_type left_cart_proj_cfunc_prod terminal_func_type)
+  qed
+
+  show "\<exists>m. m : X \<rightarrow> X \<times>\<^sub>c Y \<and> monomorphism m"
+    using mono map_type by auto
+qed
+
+lemma smaller_than_product2:
+  assumes "nonempty Y"
+  shows "X \<le>\<^sub>c Y \<times>\<^sub>c X"
+  unfolding is_smaller_than_def  
+proof - 
+  have "X \<le>\<^sub>c X \<times>\<^sub>c Y"
+    by (simp add: assms smaller_than_product1)
+  then obtain m where m_def: "m : X \<rightarrow> X \<times>\<^sub>c Y \<and> monomorphism m"
+    using is_smaller_than_def by blast
+  obtain i  where "i : (X \<times>\<^sub>c Y) \<rightarrow> (Y \<times>\<^sub>c X) \<and> isomorphism i"
+    using is_isomorphic_def product_commutes by blast
+  then have "i \<circ>\<^sub>c m : X \<rightarrow>  (Y \<times>\<^sub>c X) \<and> monomorphism(i \<circ>\<^sub>c m)"
+    using cfunc_type_def comp_type composition_of_monic_pair_is_monic iso_imp_epi_and_monic m_def by auto
+  then show "\<exists>m. m : X \<rightarrow> Y \<times>\<^sub>c X \<and> monomorphism m"
+    by blast
+qed
+
+lemma Y_nonempty_then_X_le_XtoY:
+  assumes "nonempty Y"
+  shows "X \<le>\<^sub>c X\<^bsup>Y\<^esup>"
+proof - 
+  obtain f where f_def: "f = (right_cart_proj Y X)\<^sup>\<sharp>"
+    by blast
+  then have f_type: "f : X \<rightarrow> X\<^bsup>Y\<^esup>"
+    by (simp add: right_cart_proj_type transpose_func_type)
+  have mono_f: "injective(f)"
+    unfolding injective_def
+  proof(auto)
+    fix x y 
+    assume x_type: "x \<in>\<^sub>c domain f"
+    assume y_type: "y \<in>\<^sub>c domain f"
+    assume equals: "f \<circ>\<^sub>c x = f \<circ>\<^sub>c y"
+    have x_type2 : "x \<in>\<^sub>c X"
+      using cfunc_type_def f_type x_type by auto
+    have y_type2 : "y \<in>\<^sub>c X"
+      using cfunc_type_def f_type y_type by auto
+    have "x \<circ>\<^sub>c (right_cart_proj Y one) = (right_cart_proj Y X) \<circ>\<^sub>c (id(Y) \<times>\<^sub>f x)"
+      using right_cart_proj_cfunc_cross_prod x_type2 by (typecheck_cfuncs, auto)
+    also have "... = ((eval_func X Y) \<circ>\<^sub>c (id(Y) \<times>\<^sub>f f)) \<circ>\<^sub>c (id(Y) \<times>\<^sub>f x)"
+      by (typecheck_cfuncs, simp add: f_def transpose_func_def)
+    also have "... = (eval_func X Y) \<circ>\<^sub>c ((id(Y) \<times>\<^sub>f f) \<circ>\<^sub>c (id(Y) \<times>\<^sub>f x))"
+      using comp_associative2 f_type x_type2 by (typecheck_cfuncs, fastforce)
+    also have "... = (eval_func X Y) \<circ>\<^sub>c (id(Y) \<times>\<^sub>f (f \<circ>\<^sub>c x))"
+      using f_type identity_distributes_across_composition x_type2 by auto
+    also have "... = (eval_func X Y) \<circ>\<^sub>c (id(Y) \<times>\<^sub>f (f \<circ>\<^sub>c y))"
+      by (simp add: equals)
+    also have "... = (eval_func X Y) \<circ>\<^sub>c ((id(Y) \<times>\<^sub>f f) \<circ>\<^sub>c (id(Y) \<times>\<^sub>f y))"
+      using f_type identity_distributes_across_composition y_type2 by auto
+    also have "... = ((eval_func X Y) \<circ>\<^sub>c (id(Y) \<times>\<^sub>f f)) \<circ>\<^sub>c (id(Y) \<times>\<^sub>f y)"
+      using comp_associative2 f_type y_type2 by (typecheck_cfuncs, fastforce)
+    also have "... = (right_cart_proj Y X) \<circ>\<^sub>c (id(Y) \<times>\<^sub>f y)"
+      by (typecheck_cfuncs, simp add: f_def transpose_func_def)
+    also have "... = y \<circ>\<^sub>c (right_cart_proj Y one)"
+      using right_cart_proj_cfunc_cross_prod y_type2 by (typecheck_cfuncs, auto)
+    then show "x = y"
+      using  assms calculation epimorphism_def3 nonempty_left_imp_right_proj_epimorphism right_cart_proj_type x_type2 y_type2 by fastforce
+  qed
+  then show "X \<le>\<^sub>c X\<^bsup>Y\<^esup>"
+    using f_type injective_imp_monomorphism is_smaller_than_def by blast
+qed
+
+
+
+
+
+lemma non_init_non_ter_sets:
+  assumes "\<not>(terminal_object X)"
+  assumes "\<not>(initial_object X)"
+  shows "\<Omega> \<le>\<^sub>c X" 
+proof - 
+  obtain x1 and x2 where x1_type[type_rule]: "x1 \<in>\<^sub>c X" and 
+                         x2_type[type_rule]: "x2 \<in>\<^sub>c X" and
+                                   distinct: "x1 \<noteq> x2"
+    using is_empty_def assms iso_empty_initial iso_to1_is_term no_el_iff_iso_empty single_elem_iso_one by blast
+
+
+    then have map_type: "(x1 \<amalg> x2) \<circ>\<^sub>c case_bool   : \<Omega> \<rightarrow> X"
+    by typecheck_cfuncs
+  have injective: "injective((x1 \<amalg> x2) \<circ>\<^sub>c case_bool)"
+  proof(unfold injective_def, auto)
+    fix \<omega>1 \<omega>2 
+    assume "\<omega>1 \<in>\<^sub>c domain (x1 \<amalg> x2 \<circ>\<^sub>c case_bool)"
+    then have \<omega>1_type[type_rule]: "\<omega>1 \<in>\<^sub>c \<Omega>"
+      using cfunc_type_def map_type by auto
+    assume "\<omega>2 \<in>\<^sub>c domain (x1 \<amalg> x2 \<circ>\<^sub>c case_bool)"
+    then have \<omega>2_type[type_rule]: "\<omega>2 \<in>\<^sub>c \<Omega>"
+      using cfunc_type_def map_type by auto
+    
+    assume equals: "(x1 \<amalg> x2 \<circ>\<^sub>c case_bool) \<circ>\<^sub>c \<omega>1 = (x1 \<amalg> x2 \<circ>\<^sub>c case_bool) \<circ>\<^sub>c \<omega>2"
+    show "\<omega>1 = \<omega>2"
+    proof(cases "\<omega>1 = \<t>", auto)
+      assume "\<omega>1 = \<t>"
+      show "\<t> = \<omega>2"
+      proof(rule ccontr)
+        assume " \<t> \<noteq> \<omega>2"
+        then have "\<f> = \<omega>2"
+          using \<open>\<t> \<noteq> \<omega>2\<close> true_false_only_truth_values by (typecheck_cfuncs, blast)
+        then have RHS: "(x1 \<amalg> x2 \<circ>\<^sub>c case_bool) \<circ>\<^sub>c \<omega>2 = x2"
+          by (meson coprod_case_bool_false x1_type x2_type)
+        have "(x1 \<amalg> x2 \<circ>\<^sub>c case_bool) \<circ>\<^sub>c \<omega>1 = x1"
+          using \<open>\<omega>1 = \<t>\<close> coprod_case_bool_true x1_type x2_type by blast
+        then show False
+          using RHS distinct equals by force
+      qed
+    next
+      assume "\<omega>1 \<noteq> \<t>"
+      then have "\<omega>1 = \<f>"
+        using  true_false_only_truth_values by (typecheck_cfuncs, blast)
+      have "\<omega>2 = \<f>"
+      proof(rule ccontr)
+        assume "\<omega>2 \<noteq> \<f>"
+        then have "\<omega>2 = \<t>"
+          using  true_false_only_truth_values by (typecheck_cfuncs, blast)
+        then have RHS: "(x1 \<amalg> x2 \<circ>\<^sub>c case_bool) \<circ>\<^sub>c \<omega>2 = x2"
+          using \<open>\<omega>1 = \<f>\<close> coprod_case_bool_false equals x1_type x2_type by auto
+        have "(x1 \<amalg> x2 \<circ>\<^sub>c case_bool) \<circ>\<^sub>c \<omega>1 = x1"
+          using \<open>\<omega>2 = \<t>\<close> coprod_case_bool_true equals x1_type x2_type by presburger
+        then show False
+          using RHS distinct equals by auto
+      qed
+      show "\<omega>1 = \<omega>2"
+        by (simp add: \<open>\<omega>1 = \<f>\<close> \<open>\<omega>2 = \<f>\<close>)
+    qed
+  qed
+  then have "monomorphism((x1 \<amalg> x2) \<circ>\<^sub>c case_bool)"
+    using injective_imp_monomorphism by auto
+  then show "\<Omega> \<le>\<^sub>c X"
+    using  is_smaller_than_def map_type by blast
+qed
+
+lemma exp_preserves_card1:
+  assumes "A \<le>\<^sub>c B"
+  assumes "nonempty X"   
+  shows "X\<^bsup>A\<^esup> \<le>\<^sub>c X\<^bsup>B\<^esup>"
+proof (unfold is_smaller_than_def)
+
+  obtain x where x_type[type_rule]: "x \<in>\<^sub>c X"
+    using assms(2) unfolding nonempty_def by auto
+
+  obtain m where m_def[type_rule]: "m : A \<rightarrow> B" "monomorphism m"
+    using assms(1) unfolding is_smaller_than_def by auto
+
+  show "\<exists>m. m : X\<^bsup>A\<^esup> \<rightarrow> X\<^bsup>B\<^esup> \<and> monomorphism m"
+  proof (rule_tac x="(((eval_func X A \<circ>\<^sub>c swap (X\<^bsup>A\<^esup>) A) \<amalg> (x \<circ>\<^sub>c \<beta>\<^bsub>X\<^bsup>A\<^esup> \<times>\<^sub>c (B \<setminus> (A, m))\<^esub>))
+    \<circ>\<^sub>c dist_prod_coprod_inv (X\<^bsup>A\<^esup>) A (B \<setminus> (A, m)) 
+    \<circ>\<^sub>c swap (A \<Coprod> (B \<setminus> (A, m))) (X\<^bsup>A\<^esup>) \<circ>\<^sub>c (try_cast m \<times>\<^sub>f id (X\<^bsup>A\<^esup>)))\<^sup>\<sharp>" in exI, auto)
+
+    show "((eval_func X A \<circ>\<^sub>c swap (X\<^bsup>A\<^esup>) A) \<amalg> (x \<circ>\<^sub>c \<beta>\<^bsub>X\<^bsup>A\<^esup> \<times>\<^sub>c (B \<setminus> (A, m))\<^esub>) \<circ>\<^sub>c dist_prod_coprod_inv (X\<^bsup>A\<^esup>) A (B \<setminus> (A, m)) \<circ>\<^sub>c swap (A \<Coprod> (B \<setminus> (A, m))) (X\<^bsup>A\<^esup>) \<circ>\<^sub>c try_cast m \<times>\<^sub>f id\<^sub>c (X\<^bsup>A\<^esup>))\<^sup>\<sharp> : X\<^bsup>A\<^esup> \<rightarrow> X\<^bsup>B\<^esup>"
+      by  typecheck_cfuncs
+    then show "monomorphism
+      (((eval_func X A \<circ>\<^sub>c swap (X\<^bsup>A\<^esup>) A) \<amalg> (x \<circ>\<^sub>c \<beta>\<^bsub>X\<^bsup>A\<^esup> \<times>\<^sub>c (B \<setminus> (A, m))\<^esub>) \<circ>\<^sub>c
+        dist_prod_coprod_inv (X\<^bsup>A\<^esup>) A (B \<setminus> (A, m)) \<circ>\<^sub>c
+        swap (A \<Coprod> (B \<setminus> (A, m))) (X\<^bsup>A\<^esup>) \<circ>\<^sub>c try_cast m \<times>\<^sub>f id\<^sub>c (X\<^bsup>A\<^esup>))\<^sup>\<sharp>)"
+    proof (unfold monomorphism_def3, auto)
+      fix g h Z
+      assume g_type[type_rule]: "g : Z \<rightarrow> X\<^bsup>A\<^esup>"
+      assume h_type[type_rule]: "h : Z \<rightarrow> X\<^bsup>A\<^esup>"
+      assume eq: "((eval_func X A \<circ>\<^sub>c swap (X\<^bsup>A\<^esup>) A) \<amalg> (x \<circ>\<^sub>c \<beta>\<^bsub>X\<^bsup>A\<^esup> \<times>\<^sub>c (B \<setminus> (A, m))\<^esub>) \<circ>\<^sub>c
+          dist_prod_coprod_inv (X\<^bsup>A\<^esup>) A (B \<setminus> (A, m)) \<circ>\<^sub>c
+          swap (A \<Coprod> (B \<setminus> (A, m))) (X\<^bsup>A\<^esup>) \<circ>\<^sub>c try_cast m \<times>\<^sub>f id\<^sub>c (X\<^bsup>A\<^esup>))\<^sup>\<sharp> \<circ>\<^sub>c g
+        =
+          ((eval_func X A \<circ>\<^sub>c swap (X\<^bsup>A\<^esup>) A) \<amalg> (x \<circ>\<^sub>c \<beta>\<^bsub>X\<^bsup>A\<^esup> \<times>\<^sub>c (B \<setminus> (A, m))\<^esub>) \<circ>\<^sub>c
+          dist_prod_coprod_inv (X\<^bsup>A\<^esup>) A (B \<setminus> (A, m)) \<circ>\<^sub>c
+          swap (A \<Coprod> (B \<setminus> (A, m))) (X\<^bsup>A\<^esup>) \<circ>\<^sub>c try_cast m \<times>\<^sub>f id\<^sub>c (X\<^bsup>A\<^esup>))\<^sup>\<sharp> \<circ>\<^sub>c h"
+
+      show "g = h"
+      proof (typecheck_cfuncs, rule_tac same_evals_equal[where Z=Z, where A=A, where X=X], auto)
+        show "eval_func X A \<circ>\<^sub>c id\<^sub>c A \<times>\<^sub>f g = eval_func X A \<circ>\<^sub>c id\<^sub>c A \<times>\<^sub>f h"
+        proof (typecheck_cfuncs, rule one_separator[where X="A \<times>\<^sub>c Z", where Y="X"], auto)
+          fix az
+          assume az_type[type_rule]: "az \<in>\<^sub>c A \<times>\<^sub>c Z"
+
+          obtain a z where az_types[type_rule]: "a \<in>\<^sub>c A" "z \<in>\<^sub>c Z" and az_def: "az = \<langle>a,z\<rangle>"
+            using cart_prod_decomp az_type by blast
+
+          have "(eval_func X B) \<circ>\<^sub>c (id B \<times>\<^sub>f (((eval_func X A \<circ>\<^sub>c swap (X\<^bsup>A\<^esup>) A) \<amalg> (x \<circ>\<^sub>c \<beta>\<^bsub>X\<^bsup>A\<^esup> \<times>\<^sub>c (B \<setminus> (A, m))\<^esub>) \<circ>\<^sub>c
+            dist_prod_coprod_inv (X\<^bsup>A\<^esup>) A (B \<setminus> (A, m)) \<circ>\<^sub>c
+            swap (A \<Coprod> (B \<setminus> (A, m))) (X\<^bsup>A\<^esup>) \<circ>\<^sub>c try_cast m \<times>\<^sub>f id\<^sub>c (X\<^bsup>A\<^esup>))\<^sup>\<sharp> \<circ>\<^sub>c g)) = 
+          (eval_func X B) \<circ>\<^sub>c (id B \<times>\<^sub>f (((eval_func X A \<circ>\<^sub>c swap (X\<^bsup>A\<^esup>) A) \<amalg> (x \<circ>\<^sub>c \<beta>\<^bsub>X\<^bsup>A\<^esup> \<times>\<^sub>c (B \<setminus> (A, m))\<^esub>) \<circ>\<^sub>c
+            dist_prod_coprod_inv (X\<^bsup>A\<^esup>) A (B \<setminus> (A, m)) \<circ>\<^sub>c
+            swap (A \<Coprod> (B \<setminus> (A, m))) (X\<^bsup>A\<^esup>) \<circ>\<^sub>c try_cast m \<times>\<^sub>f id\<^sub>c (X\<^bsup>A\<^esup>))\<^sup>\<sharp> \<circ>\<^sub>c h))"
+            using eq by simp
+          then have "(eval_func X B)\<circ>\<^sub>c (id B \<times>\<^sub>f (((eval_func X A \<circ>\<^sub>c swap (X\<^bsup>A\<^esup>) A) \<amalg> (x \<circ>\<^sub>c \<beta>\<^bsub>X\<^bsup>A\<^esup> \<times>\<^sub>c (B \<setminus> (A, m))\<^esub>) \<circ>\<^sub>c
+            dist_prod_coprod_inv (X\<^bsup>A\<^esup>) A (B \<setminus> (A, m)) \<circ>\<^sub>c
+            swap (A \<Coprod> (B \<setminus> (A, m))) (X\<^bsup>A\<^esup>) \<circ>\<^sub>c try_cast m \<times>\<^sub>f id\<^sub>c (X\<^bsup>A\<^esup>))\<^sup>\<sharp>)) \<circ>\<^sub>c (id B \<times>\<^sub>f  g) = 
+          (eval_func X B)\<circ>\<^sub>c (id B \<times>\<^sub>f (((eval_func X A \<circ>\<^sub>c swap (X\<^bsup>A\<^esup>) A) \<amalg> (x \<circ>\<^sub>c \<beta>\<^bsub>X\<^bsup>A\<^esup> \<times>\<^sub>c (B \<setminus> (A, m))\<^esub>) \<circ>\<^sub>c
+            dist_prod_coprod_inv (X\<^bsup>A\<^esup>) A (B \<setminus> (A, m)) \<circ>\<^sub>c
+            swap (A \<Coprod> (B \<setminus> (A, m))) (X\<^bsup>A\<^esup>) \<circ>\<^sub>c try_cast m \<times>\<^sub>f id\<^sub>c (X\<^bsup>A\<^esup>))\<^sup>\<sharp>)) \<circ>\<^sub>c (id B \<times>\<^sub>f  h)"
+            using identity_distributes_across_composition by (typecheck_cfuncs, auto)
+          then have "((eval_func X B)\<circ>\<^sub>c (id B \<times>\<^sub>f (((eval_func X A \<circ>\<^sub>c swap (X\<^bsup>A\<^esup>) A) \<amalg> (x \<circ>\<^sub>c \<beta>\<^bsub>X\<^bsup>A\<^esup> \<times>\<^sub>c (B \<setminus> (A, m))\<^esub>) \<circ>\<^sub>c
+            dist_prod_coprod_inv (X\<^bsup>A\<^esup>) A (B \<setminus> (A, m)) \<circ>\<^sub>c
+            swap (A \<Coprod> (B \<setminus> (A, m))) (X\<^bsup>A\<^esup>) \<circ>\<^sub>c try_cast m \<times>\<^sub>f id\<^sub>c (X\<^bsup>A\<^esup>))\<^sup>\<sharp>))) \<circ>\<^sub>c (id B \<times>\<^sub>f  g) = 
+          ((eval_func X B)\<circ>\<^sub>c (id B \<times>\<^sub>f (((eval_func X A \<circ>\<^sub>c swap (X\<^bsup>A\<^esup>) A) \<amalg> (x \<circ>\<^sub>c \<beta>\<^bsub>X\<^bsup>A\<^esup> \<times>\<^sub>c (B \<setminus> (A, m))\<^esub>) \<circ>\<^sub>c
+            dist_prod_coprod_inv (X\<^bsup>A\<^esup>) A (B \<setminus> (A, m)) \<circ>\<^sub>c
+            swap (A \<Coprod> (B \<setminus> (A, m))) (X\<^bsup>A\<^esup>) \<circ>\<^sub>c try_cast m \<times>\<^sub>f id\<^sub>c (X\<^bsup>A\<^esup>))\<^sup>\<sharp>))) \<circ>\<^sub>c (id B \<times>\<^sub>f  h)"
+            by (typecheck_cfuncs, smt eq inv_transpose_func_def3 inv_transpose_of_composition)
+          then have "((eval_func X A \<circ>\<^sub>c swap (X\<^bsup>A\<^esup>) A) \<amalg> (x \<circ>\<^sub>c \<beta>\<^bsub>X\<^bsup>A\<^esup> \<times>\<^sub>c (B \<setminus> (A, m))\<^esub>) \<circ>\<^sub>c
+            dist_prod_coprod_inv (X\<^bsup>A\<^esup>) A (B \<setminus> (A, m)) \<circ>\<^sub>c
+            swap (A \<Coprod> (B \<setminus> (A, m))) (X\<^bsup>A\<^esup>) \<circ>\<^sub>c try_cast m \<times>\<^sub>f id\<^sub>c (X\<^bsup>A\<^esup>)) \<circ>\<^sub>c (id B \<times>\<^sub>f  g)
+          = ((eval_func X A \<circ>\<^sub>c swap (X\<^bsup>A\<^esup>) A) \<amalg> (x \<circ>\<^sub>c \<beta>\<^bsub>X\<^bsup>A\<^esup> \<times>\<^sub>c (B \<setminus> (A, m))\<^esub>) \<circ>\<^sub>c
+            dist_prod_coprod_inv (X\<^bsup>A\<^esup>) A (B \<setminus> (A, m)) \<circ>\<^sub>c
+            swap (A \<Coprod> (B \<setminus> (A, m))) (X\<^bsup>A\<^esup>) \<circ>\<^sub>c try_cast m \<times>\<^sub>f id\<^sub>c (X\<^bsup>A\<^esup>)) \<circ>\<^sub>c (id B \<times>\<^sub>f  h)"
+            using   transpose_func_def by (typecheck_cfuncs,auto)
+          then have "(((eval_func X A \<circ>\<^sub>c swap (X\<^bsup>A\<^esup>) A) \<amalg> (x \<circ>\<^sub>c \<beta>\<^bsub>X\<^bsup>A\<^esup> \<times>\<^sub>c (B \<setminus> (A, m))\<^esub>) \<circ>\<^sub>c
+            dist_prod_coprod_inv (X\<^bsup>A\<^esup>) A (B \<setminus> (A, m)) \<circ>\<^sub>c
+            swap (A \<Coprod> (B \<setminus> (A, m))) (X\<^bsup>A\<^esup>) \<circ>\<^sub>c try_cast m \<times>\<^sub>f id\<^sub>c (X\<^bsup>A\<^esup>)) \<circ>\<^sub>c (id B \<times>\<^sub>f  g)) \<circ>\<^sub>c \<langle>m \<circ>\<^sub>c a, z\<rangle>
+          = (((eval_func X A \<circ>\<^sub>c swap (X\<^bsup>A\<^esup>) A) \<amalg> (x \<circ>\<^sub>c \<beta>\<^bsub>X\<^bsup>A\<^esup> \<times>\<^sub>c (B \<setminus> (A, m))\<^esub>) \<circ>\<^sub>c
+            dist_prod_coprod_inv (X\<^bsup>A\<^esup>) A (B \<setminus> (A, m)) \<circ>\<^sub>c
+            swap (A \<Coprod> (B \<setminus> (A, m))) (X\<^bsup>A\<^esup>) \<circ>\<^sub>c try_cast m \<times>\<^sub>f id\<^sub>c (X\<^bsup>A\<^esup>)) \<circ>\<^sub>c (id B \<times>\<^sub>f  h)) \<circ>\<^sub>c \<langle>m \<circ>\<^sub>c a, z\<rangle>"
+            by auto
+          then have "((eval_func X A \<circ>\<^sub>c swap (X\<^bsup>A\<^esup>) A) \<amalg> (x \<circ>\<^sub>c \<beta>\<^bsub>X\<^bsup>A\<^esup> \<times>\<^sub>c (B \<setminus> (A, m))\<^esub>) \<circ>\<^sub>c
+            dist_prod_coprod_inv (X\<^bsup>A\<^esup>) A (B \<setminus> (A, m)) \<circ>\<^sub>c
+            swap (A \<Coprod> (B \<setminus> (A, m))) (X\<^bsup>A\<^esup>) \<circ>\<^sub>c try_cast m \<times>\<^sub>f id\<^sub>c (X\<^bsup>A\<^esup>)) \<circ>\<^sub>c (id B \<times>\<^sub>f  g) \<circ>\<^sub>c \<langle>m \<circ>\<^sub>c a, z\<rangle>
+          = ((eval_func X A \<circ>\<^sub>c swap (X\<^bsup>A\<^esup>) A) \<amalg> (x \<circ>\<^sub>c \<beta>\<^bsub>X\<^bsup>A\<^esup> \<times>\<^sub>c (B \<setminus> (A, m))\<^esub>) \<circ>\<^sub>c
+            dist_prod_coprod_inv (X\<^bsup>A\<^esup>) A (B \<setminus> (A, m)) \<circ>\<^sub>c
+            swap (A \<Coprod> (B \<setminus> (A, m))) (X\<^bsup>A\<^esup>) \<circ>\<^sub>c try_cast m \<times>\<^sub>f id\<^sub>c (X\<^bsup>A\<^esup>)) \<circ>\<^sub>c (id B \<times>\<^sub>f  h) \<circ>\<^sub>c \<langle>m \<circ>\<^sub>c a, z\<rangle>"
+            by (typecheck_cfuncs, auto simp add: comp_associative2)
+          then have "((eval_func X A \<circ>\<^sub>c swap (X\<^bsup>A\<^esup>) A) \<amalg> (x \<circ>\<^sub>c \<beta>\<^bsub>X\<^bsup>A\<^esup> \<times>\<^sub>c (B \<setminus> (A, m))\<^esub>) \<circ>\<^sub>c
+            dist_prod_coprod_inv (X\<^bsup>A\<^esup>) A (B \<setminus> (A, m)) \<circ>\<^sub>c
+            swap (A \<Coprod> (B \<setminus> (A, m))) (X\<^bsup>A\<^esup>) \<circ>\<^sub>c try_cast m \<times>\<^sub>f id\<^sub>c (X\<^bsup>A\<^esup>)) \<circ>\<^sub>c \<langle>m \<circ>\<^sub>c a, g \<circ>\<^sub>c z\<rangle>
+          = ((eval_func X A \<circ>\<^sub>c swap (X\<^bsup>A\<^esup>) A) \<amalg> (x \<circ>\<^sub>c \<beta>\<^bsub>X\<^bsup>A\<^esup> \<times>\<^sub>c (B \<setminus> (A, m))\<^esub>) \<circ>\<^sub>c
+            dist_prod_coprod_inv (X\<^bsup>A\<^esup>) A (B \<setminus> (A, m)) \<circ>\<^sub>c
+            swap (A \<Coprod> (B \<setminus> (A, m))) (X\<^bsup>A\<^esup>) \<circ>\<^sub>c try_cast m \<times>\<^sub>f id\<^sub>c (X\<^bsup>A\<^esup>)) \<circ>\<^sub>c \<langle>m \<circ>\<^sub>c a, h \<circ>\<^sub>c z\<rangle>"
+            by (typecheck_cfuncs, smt cfunc_cross_prod_comp_cfunc_prod id_left_unit2 id_type)
+          then have "(eval_func X A \<circ>\<^sub>c swap (X\<^bsup>A\<^esup>) A) \<amalg> (x \<circ>\<^sub>c \<beta>\<^bsub>X\<^bsup>A\<^esup> \<times>\<^sub>c (B \<setminus> (A, m))\<^esub>) \<circ>\<^sub>c
+            dist_prod_coprod_inv (X\<^bsup>A\<^esup>) A (B \<setminus> (A, m)) \<circ>\<^sub>c
+            swap (A \<Coprod> (B \<setminus> (A, m))) (X\<^bsup>A\<^esup>) \<circ>\<^sub>c (try_cast m \<times>\<^sub>f id\<^sub>c (X\<^bsup>A\<^esup>)) \<circ>\<^sub>c \<langle>m \<circ>\<^sub>c a, g \<circ>\<^sub>c z\<rangle>
+          = (eval_func X A \<circ>\<^sub>c swap (X\<^bsup>A\<^esup>) A) \<amalg> (x \<circ>\<^sub>c \<beta>\<^bsub>X\<^bsup>A\<^esup> \<times>\<^sub>c (B \<setminus> (A, m))\<^esub>) \<circ>\<^sub>c
+            dist_prod_coprod_inv (X\<^bsup>A\<^esup>) A (B \<setminus> (A, m)) \<circ>\<^sub>c
+            swap (A \<Coprod> (B \<setminus> (A, m))) (X\<^bsup>A\<^esup>) \<circ>\<^sub>c (try_cast m \<times>\<^sub>f id\<^sub>c (X\<^bsup>A\<^esup>)) \<circ>\<^sub>c \<langle>m \<circ>\<^sub>c a, h \<circ>\<^sub>c z\<rangle>"
+            by (typecheck_cfuncs_prems, smt comp_associative2)
+          then have "(eval_func X A \<circ>\<^sub>c swap (X\<^bsup>A\<^esup>) A) \<amalg> (x \<circ>\<^sub>c \<beta>\<^bsub>X\<^bsup>A\<^esup> \<times>\<^sub>c (B \<setminus> (A, m))\<^esub>) \<circ>\<^sub>c
+            dist_prod_coprod_inv (X\<^bsup>A\<^esup>) A (B \<setminus> (A, m)) \<circ>\<^sub>c
+            swap (A \<Coprod> (B \<setminus> (A, m))) (X\<^bsup>A\<^esup>) \<circ>\<^sub>c \<langle>try_cast m \<circ>\<^sub>c m \<circ>\<^sub>c a, g \<circ>\<^sub>c z\<rangle>
+          = (eval_func X A \<circ>\<^sub>c swap (X\<^bsup>A\<^esup>) A) \<amalg> (x \<circ>\<^sub>c \<beta>\<^bsub>X\<^bsup>A\<^esup> \<times>\<^sub>c (B \<setminus> (A, m))\<^esub>) \<circ>\<^sub>c
+            dist_prod_coprod_inv (X\<^bsup>A\<^esup>) A (B \<setminus> (A, m)) \<circ>\<^sub>c
+            swap (A \<Coprod> (B \<setminus> (A, m))) (X\<^bsup>A\<^esup>) \<circ>\<^sub>c \<langle>try_cast m \<circ>\<^sub>c m \<circ>\<^sub>c a, h \<circ>\<^sub>c z\<rangle>"
+            using cfunc_cross_prod_comp_cfunc_prod id_left_unit2 by (typecheck_cfuncs_prems, smt)
+          then have "(eval_func X A \<circ>\<^sub>c swap (X\<^bsup>A\<^esup>) A) \<amalg> (x \<circ>\<^sub>c \<beta>\<^bsub>X\<^bsup>A\<^esup> \<times>\<^sub>c (B \<setminus> (A, m))\<^esub>) \<circ>\<^sub>c
+            dist_prod_coprod_inv (X\<^bsup>A\<^esup>) A (B \<setminus> (A, m)) \<circ>\<^sub>c
+            swap (A \<Coprod> (B \<setminus> (A, m))) (X\<^bsup>A\<^esup>) \<circ>\<^sub>c \<langle>(try_cast m \<circ>\<^sub>c m) \<circ>\<^sub>c a, g \<circ>\<^sub>c z\<rangle>
+          = (eval_func X A \<circ>\<^sub>c swap (X\<^bsup>A\<^esup>) A) \<amalg> (x \<circ>\<^sub>c \<beta>\<^bsub>X\<^bsup>A\<^esup> \<times>\<^sub>c (B \<setminus> (A, m))\<^esub>) \<circ>\<^sub>c
+            dist_prod_coprod_inv (X\<^bsup>A\<^esup>) A (B \<setminus> (A, m)) \<circ>\<^sub>c
+            swap (A \<Coprod> (B \<setminus> (A, m))) (X\<^bsup>A\<^esup>) \<circ>\<^sub>c \<langle>(try_cast m \<circ>\<^sub>c m) \<circ>\<^sub>c a, h \<circ>\<^sub>c z\<rangle>"
+            by (typecheck_cfuncs, auto simp add: comp_associative2)
+          then have "(eval_func X A \<circ>\<^sub>c swap (X\<^bsup>A\<^esup>) A) \<amalg> (x \<circ>\<^sub>c \<beta>\<^bsub>X\<^bsup>A\<^esup> \<times>\<^sub>c (B \<setminus> (A, m))\<^esub>) \<circ>\<^sub>c
+            dist_prod_coprod_inv (X\<^bsup>A\<^esup>) A (B \<setminus> (A, m)) \<circ>\<^sub>c
+            swap (A \<Coprod> (B \<setminus> (A, m))) (X\<^bsup>A\<^esup>) \<circ>\<^sub>c \<langle>left_coproj A (B \<setminus> (A,m)) \<circ>\<^sub>c a, g \<circ>\<^sub>c z\<rangle>
+          = (eval_func X A \<circ>\<^sub>c swap (X\<^bsup>A\<^esup>) A) \<amalg> (x \<circ>\<^sub>c \<beta>\<^bsub>X\<^bsup>A\<^esup> \<times>\<^sub>c (B \<setminus> (A, m))\<^esub>) \<circ>\<^sub>c
+            dist_prod_coprod_inv (X\<^bsup>A\<^esup>) A (B \<setminus> (A, m)) \<circ>\<^sub>c
+            swap (A \<Coprod> (B \<setminus> (A, m))) (X\<^bsup>A\<^esup>) \<circ>\<^sub>c \<langle>left_coproj A (B \<setminus> (A,m)) \<circ>\<^sub>c a, h \<circ>\<^sub>c z\<rangle>"
+            using m_def(2) try_cast_m_m by (typecheck_cfuncs, auto)
+          then have "(eval_func X A \<circ>\<^sub>c swap (X\<^bsup>A\<^esup>) A) \<amalg> (x \<circ>\<^sub>c \<beta>\<^bsub>X\<^bsup>A\<^esup> \<times>\<^sub>c (B \<setminus> (A, m))\<^esub>) \<circ>\<^sub>c
+            dist_prod_coprod_inv (X\<^bsup>A\<^esup>) A (B \<setminus> (A, m)) \<circ>\<^sub>c \<langle>g \<circ>\<^sub>c z, left_coproj A (B \<setminus> (A,m)) \<circ>\<^sub>c a\<rangle>
+          = (eval_func X A \<circ>\<^sub>c swap (X\<^bsup>A\<^esup>) A) \<amalg> (x \<circ>\<^sub>c \<beta>\<^bsub>X\<^bsup>A\<^esup> \<times>\<^sub>c (B \<setminus> (A, m))\<^esub>) \<circ>\<^sub>c
+            dist_prod_coprod_inv (X\<^bsup>A\<^esup>) A (B \<setminus> (A, m)) \<circ>\<^sub>c \<langle>h \<circ>\<^sub>c z, left_coproj A (B \<setminus> (A,m)) \<circ>\<^sub>c a\<rangle>"
+            using swap_ap by (typecheck_cfuncs, auto)
+          then have "(eval_func X A \<circ>\<^sub>c swap (X\<^bsup>A\<^esup>) A) \<amalg> (x \<circ>\<^sub>c \<beta>\<^bsub>X\<^bsup>A\<^esup> \<times>\<^sub>c (B \<setminus> (A, m))\<^esub>) \<circ>\<^sub>c
+            left_coproj (X\<^bsup>A\<^esup>\<times>\<^sub>cA) (X\<^bsup>A\<^esup>\<times>\<^sub>c(B \<setminus> (A,m))) \<circ>\<^sub>c \<langle>g \<circ>\<^sub>c z, a\<rangle>
+          = (eval_func X A \<circ>\<^sub>c swap (X\<^bsup>A\<^esup>) A) \<amalg> (x \<circ>\<^sub>c \<beta>\<^bsub>X\<^bsup>A\<^esup> \<times>\<^sub>c (B \<setminus> (A, m))\<^esub>) \<circ>\<^sub>c
+            left_coproj (X\<^bsup>A\<^esup>\<times>\<^sub>cA) (X\<^bsup>A\<^esup>\<times>\<^sub>c(B \<setminus> (A,m))) \<circ>\<^sub>c \<langle>h \<circ>\<^sub>c z,a\<rangle>"
+            using dist_prod_coprod_inv_left_ap by (typecheck_cfuncs, auto)
+          then have "((eval_func X A \<circ>\<^sub>c swap (X\<^bsup>A\<^esup>) A) \<amalg> (x \<circ>\<^sub>c \<beta>\<^bsub>X\<^bsup>A\<^esup> \<times>\<^sub>c (B \<setminus> (A, m))\<^esub>) \<circ>\<^sub>c
+            left_coproj (X\<^bsup>A\<^esup>\<times>\<^sub>cA) (X\<^bsup>A\<^esup>\<times>\<^sub>c(B \<setminus> (A,m)))) \<circ>\<^sub>c \<langle>g \<circ>\<^sub>c z, a\<rangle>
+          = ((eval_func X A \<circ>\<^sub>c swap (X\<^bsup>A\<^esup>) A) \<amalg> (x \<circ>\<^sub>c \<beta>\<^bsub>X\<^bsup>A\<^esup> \<times>\<^sub>c (B \<setminus> (A, m))\<^esub>) \<circ>\<^sub>c
+            left_coproj (X\<^bsup>A\<^esup>\<times>\<^sub>cA) (X\<^bsup>A\<^esup>\<times>\<^sub>c(B \<setminus> (A,m)))) \<circ>\<^sub>c \<langle>h \<circ>\<^sub>c z,a\<rangle>"
+            by (typecheck_cfuncs_prems, auto simp add: comp_associative2)
+          then have "(eval_func X A \<circ>\<^sub>c swap (X\<^bsup>A\<^esup>) A) \<circ>\<^sub>c \<langle>g \<circ>\<^sub>c z, a\<rangle>
+            = (eval_func X A \<circ>\<^sub>c swap (X\<^bsup>A\<^esup>) A) \<circ>\<^sub>c \<langle>h \<circ>\<^sub>c z,a\<rangle>"
+            by (typecheck_cfuncs_prems, auto simp add: left_coproj_cfunc_coprod)
+          then have "eval_func X A \<circ>\<^sub>c swap (X\<^bsup>A\<^esup>) A \<circ>\<^sub>c \<langle>g \<circ>\<^sub>c z, a\<rangle>
+            = eval_func X A \<circ>\<^sub>c swap (X\<^bsup>A\<^esup>) A \<circ>\<^sub>c \<langle>h \<circ>\<^sub>c z,a\<rangle>"
+            by (typecheck_cfuncs_prems, auto simp add: comp_associative2)
+          then have "eval_func X A \<circ>\<^sub>c \<langle>a, g \<circ>\<^sub>c z\<rangle> = eval_func X A \<circ>\<^sub>c \<langle>a, h \<circ>\<^sub>c z\<rangle>"
+            by (typecheck_cfuncs_prems, auto simp add: swap_ap)
+          then have "eval_func X A \<circ>\<^sub>c (id A \<times>\<^sub>f g) \<circ>\<^sub>c \<langle>a, z\<rangle> = eval_func X A \<circ>\<^sub>c (id A \<times>\<^sub>f h) \<circ>\<^sub>c \<langle>a, z\<rangle>"
+            by (typecheck_cfuncs, simp add: cfunc_cross_prod_comp_cfunc_prod id_left_unit2)
+          then show "(eval_func X A \<circ>\<^sub>c id\<^sub>c A \<times>\<^sub>f g) \<circ>\<^sub>c az = (eval_func X A \<circ>\<^sub>c id\<^sub>c A \<times>\<^sub>f h) \<circ>\<^sub>c az"
+            unfolding az_def by (typecheck_cfuncs_prems, auto simp add: comp_associative2)
+        qed
+      qed
+    qed
+  qed
+qed
+
+lemma exp_preserves_card2:
+  assumes "A \<le>\<^sub>c B"
+  shows "A\<^bsup>X\<^esup> \<le>\<^sub>c B\<^bsup>X\<^esup>"
+proof (unfold is_smaller_than_def)
+  obtain m where m_def[type_rule]: "m : A \<rightarrow> B" "monomorphism m"
+        using assms unfolding is_smaller_than_def by auto
+  show "\<exists>m. m : A\<^bsup>X\<^esup> \<rightarrow> B\<^bsup>X\<^esup> \<and> monomorphism m"
+  proof (rule_tac x="(m \<circ>\<^sub>c eval_func A X)\<^sup>\<sharp>" in exI, auto)
+    show "(m \<circ>\<^sub>c eval_func A X)\<^sup>\<sharp> : A\<^bsup>X\<^esup> \<rightarrow> B\<^bsup>X\<^esup>"
+      by typecheck_cfuncs
+    then show "monomorphism((m \<circ>\<^sub>c eval_func A X)\<^sup>\<sharp>)"
+    proof (unfold monomorphism_def3, auto)
+      fix g h Z
+      assume g_type[type_rule]: "g : Z \<rightarrow> A\<^bsup>X\<^esup>"
+      assume h_type[type_rule]: "h : Z \<rightarrow> A\<^bsup>X\<^esup>"
+
+      assume eq: "(m \<circ>\<^sub>c eval_func A X)\<^sup>\<sharp> \<circ>\<^sub>c g = (m \<circ>\<^sub>c eval_func A X)\<^sup>\<sharp> \<circ>\<^sub>c h"
+      show "g = h"
+      proof (typecheck_cfuncs, rule_tac same_evals_equal[where Z=Z, where A=X, where X=A], auto)
+          have "((eval_func B X) \<circ>\<^sub>c (id X \<times>\<^sub>f (m \<circ>\<^sub>c eval_func A X)\<^sup>\<sharp>)) \<circ>\<^sub>c (id X \<times>\<^sub>f g)  = 
+                ((eval_func B X) \<circ>\<^sub>c (id X \<times>\<^sub>f (m \<circ>\<^sub>c eval_func A X)\<^sup>\<sharp>)) \<circ>\<^sub>c (id X \<times>\<^sub>f h)"
+            by (typecheck_cfuncs, smt comp_associative2 eq inv_transpose_func_def3 inv_transpose_of_composition)
+          then have "(m \<circ>\<^sub>c eval_func A X) \<circ>\<^sub>c (id X \<times>\<^sub>f g)  = (m \<circ>\<^sub>c eval_func A X) \<circ>\<^sub>c (id X \<times>\<^sub>f h)"
+            by (smt comp_type eval_func_type m_def(1) transpose_func_def)
+          then have "m \<circ>\<^sub>c (eval_func A X \<circ>\<^sub>c (id X \<times>\<^sub>f g))  = m \<circ>\<^sub>c (eval_func A X \<circ>\<^sub>c (id X \<times>\<^sub>f h))"
+            by (typecheck_cfuncs, smt comp_associative2)
+          then have "eval_func A X \<circ>\<^sub>c (id X \<times>\<^sub>f g)  = eval_func A X \<circ>\<^sub>c (id X \<times>\<^sub>f h)"
+            using m_def monomorphism_def3 by (typecheck_cfuncs, blast)
+          then show "(eval_func A X \<circ>\<^sub>c (id X \<times>\<^sub>f g))  = (eval_func A X \<circ>\<^sub>c (id X \<times>\<^sub>f h))"
+            by (typecheck_cfuncs, smt comp_associative2)
+      qed
+    qed
+  qed
+qed
+
+lemma exp_preserves_card3:
+  assumes "A \<le>\<^sub>c B"
+  assumes "X \<le>\<^sub>c Y"
+  assumes "nonempty(X)"
+  shows "X\<^bsup>A\<^esup> \<le>\<^sub>c Y\<^bsup>B\<^esup>"
+proof - 
+  have leq1: "X\<^bsup>A\<^esup> \<le>\<^sub>c X\<^bsup>B\<^esup>"
+    by (simp add: assms(1,3) exp_preserves_card1)    
+  have leq2: "X\<^bsup>B\<^esup> \<le>\<^sub>c Y\<^bsup>B\<^esup>"
+    by (simp add: assms(2) exp_preserves_card2)
+  show "X\<^bsup>A\<^esup> \<le>\<^sub>c Y\<^bsup>B\<^esup>"
+    using leq1 leq2 set_card_transitive by blast
+qed
+
 section \<open>Zero and Successor\<close>
 
 lemma zero_is_not_successor:
@@ -375,6 +859,10 @@ proof -
   then show "injective successor \<and> \<not> surjective successor"
     using monomorphism_imp_injective succ_mono by blast
 qed
+
+corollary nat_is_infinite:
+  "is_infinite \<nat>\<^sub>c"
+  unfolding is_infinite_def using Peano's_Axioms injective_imp_monomorphism successor_type by blast
 
 lemma succ_inject:
   assumes "n \<in>\<^sub>c \<nat>\<^sub>c" "m \<in>\<^sub>c \<nat>\<^sub>c"
